\documentclass[12pt]{article}

\setlength\parindent{0pt}
\newcommand{\myt}[1]{\textbf{\underline{#1}}}

\usepackage{mathtools}
\usepackage{amssymb}
\usepackage{graphicx}

\title{\vspace{-15ex}Solving Inhomogeneous Linear Equations\vspace{-1ex}}
\date{Feb 6th, 2017}
\author{Graham Cooper}

\begin{document}
	\maketitle
	
	\subsection*{Method 1: Method of Undetermined Coefficients}
	\subsubsection*{Eg1:}
	$$y'' + 2y' - 3y = e^x$$
	Find $y_h$ the character equation is $m^2 + 2m - 3 = 0$, m = 1, -3\\
	$$y_h = C_1e^x + C_2e^{-3x}$$
	
	For $y_p$ we guess $y = Axe^x$\\
	$y' = Ae^x + Axe^x$\\
	$y'' = 2Ae^x + Axe^x$\\
	
	Plug this into the DE: $(2Ae^x + Axe^x) + 2(Ae^x + Axe^x) - 3Axe^x = e^x$\\
	$\rightarrow 4A = 1$, so $A = \frac{1}{4}$\\
	and $y = C_1e^x + C_2e^{-3x} + \frac{1}{4xe^x}$\\
	
	\subsection*{Method 2: Variation of Parameters}
	Given: $y'' + p(x)y' q(x)y = F(x)$\\
	With homogeneous solution:\\
	$y_h = C_1y_1(x) + C_2y_2(x)$\\
	We assume that the solution can be written as:\\
	$y = u_1(x)y_1(x) + u_2(x)y_2(x)$\\
	
	Differentiate:\\
	$y' = u_1'y_1 + u_1y_1' + u_2'y_2 + u_2y_2'$\\
	
	We have the freedom to impose a condition, since we have 2 unknown functions and only one condition (the DE).\\
	As the second condition set:\\
	$$u_1'y_1 + u_2'y_2 = 0$$
	$$\rightarrow y' = u_1y_1' + u_2y_2'$$
	Differentiate:\\
	$$y'' = u_1'y_1' + u_1y_1''+u_2'y_2'+u_2y_2''$$
	Plug $y'', y', y$ into the DE:\\
	$$(u_1'y_1' + u_1y_1'' + u_2'y_2' + u_2y_2'') + p(x)(u_1y_1' + u_2y_2') + g(x)(u_1y_1 + u_2y_2) = F(x)$$
	$$\rightarrow u_1'y_1'+u_2'y_2' + u_1[y_1''+p(x)y_1' + q(x)y_1] + u_2[y_2''+p(x)y_2' + q(x)y_2] = F(x)$$
	$$\rightarrow u_1'y_1' + u_2'y_2' = F(x)$$
	We were able to get rid of the bracketed parts because we are looking at our inhomogeneous case which means the original equation is equal to 0\\
	
	We can solve for $u_1'$ and $u_2'$ and then integrate!\\
	
	\subsubsection*{Example1}
	$y'' + 2y' - 3y = e^x$\\
	
	We know $y_h = C_1e^x + C_2e^{-3x}$\\
	We let: $y = u_1(X)e^x + u_2(x)e^{-3x}$\\
	To find $u_1$, $u_2$ solve:\\
	$$u_1'y_1 + u_2'y_2 = 0$$
	$$u_1'y_1' + u_2'y_2' = F(x)$$
	ie:\\
	$$u_1'e^x + u_2'e^{-3x} = 0$$
	$$u_1'e^x - 3u_2'e^{-3x} = e^x$$
	
	Isolate one of the unknowns.\\
	Subtract:\\
	$$4u_2'e^{-3x} = -e^x$$
	$$\rightarrow u_2' = \frac{-1}{4}e^{4x}$$
	$$\rightarrow u_2 = \frac{-1}{16}e^{4x} + C_2$$
	Now solve for $u_1$\\
	$$u_1'e^x = -u_2'e^{-3x}$$
	$$= \frac{1}{4}e^x$$
	$$u_1' = \frac{1}{4}$$
	$$u_1 = \frac{1}{4}x + C_1$$
	Plug these into the above equations:\\
	$$y = u_1e^x + u_2e^{-3x}$$
	$$= (\frac{1}{4}x + C_1)e^x + (\frac{-1}{16}e^{4x} + C_2)e^{-3x}$$
	$$= C_1e^x + C_2e^{-3x} + \frac{1}{4}xe^x - \frac{1}{16}e^x$$
	$$= C_3e^x + C_2e^{-3x} + \frac{1}{4}xe^x$$
	
	\subsubsection*{Example2}
	Solve the IVP $y'' + 4y = \frac{1}{x}$ for $y(\pi) = 0$ and $y'(\pi) = 0$\\
	Here $y_h = C_1cos(2x) + C_2sin(2x)$\\
	We look for $y = u_1(x)cos(2x) + u_2sin(2x)$\\
	Solve: $u_1'cos(2x) + u_2'sin(2x) = 0$\\
	$-2u_1'sin(2x) + 2u_2'cos(2x) = \frac{1}{x}$\\
	Multiply 1 by $2cos(2x)$ and 2 by $sin(2x)$ then subtract:\\
	
	$$u_1'(2cos^2(2x) + 2sin^2(2x) = \frac{-sin(2x)}{x}$$
	$$\rightarrow u_1' = \frac{-sin(2x)}{2x}$$
	$$\rightarrow u_1 = -\int_{\pi}^{x}\frac{sin(2t)}{2t}dt + C_1$$
	To find $u_2$? Equation 1 gives:\\
	$$u_2'sin(2x) = -u_1'cos(2x)$$
	$$= \frac{sin(2x)cos(2x)}{2x}$$
	$$\rightarrow u_2' = \frac{cos(2x)}{2x}$$
	$$\rightarrow u_2 = \int_{\pi}^{x}\frac{cos(2t)}{2t}dt$$
	The full solution is:\\
	$$y = C_1cos(2x) + C_2sin(2x) + cos(2x)\int_{pi}^{x}\frac{sin(2t)}{2t}dt - sin(2x)\int_{\pi}^{x}\frac{cos(2t)}{2t}dt$$
	
	To use the IC's, we need the derivitive:\\
	$$y' = -2C_1sin(2x) + 2C_2cos(2x) + \frac{cos(2x)sin(2x)}{2x} - 2sin(2x) \int_{\pi}^{x}\frac{sin(2t)}{2t}dt - \frac{sin(2x)cos(2x)}{2x} - cos(2x)\int_{\pi}{x}\frac{cos(2t)}{2t}dt$$
	$y(\pi) = C_1 = 0$ and $y'(\pi) = 2C_2 = 0$ which means $C_1 = C_2 = 0$\\
	
	$$\rightarrow y = \frac{cos(2x)}{2}\int_{\pi}^{x}\frac{sin(2t)}{t}dt - \frac{sin(2x)}{2}\int_{\pi}^{x}\frac{cos(2t)}{t}dt$$
	
	
\end{document}
